Freigen/ITree/Basic.lean
@@ -1,170 +1,57 @@
 import Freigen.IxPoly.Basic
+import Freigen.Eff
 
-namespace Freigen.ITree
+namespace Freigen
 
-open Freigen.IxPoly
-
-structure EffSpec where
-  tag : Type u
-  input : tag → Type v
-  output : tag → Type v
-  blockTag : tag → Type u
-  blockInputs : (t : tag) → blockTag t → Type v
-  blockOutputs : (t : tag) → blockTag t → Type v
-
-inductive NodeTag (E : EffSpec) : Type _ → Type _ where
-| ret {R} : R → NodeTag E R
-| tau {R} : NodeTag E R
-| fail {R} : NodeTag E R
-| op {R} (e : E.tag) : E.input e → NodeTag E R
-
-def NodeTag.fields {i} {E : EffSpec}: NodeTag E i → Type _
-| ret _ => PEmpty
-| tau => PUnit
-| fail => PEmpty
-| op e _ => E.output e ⊕ ((t : E.blockTag e) × E.blockInputs e t)
-
-def NodeTag.elem {E : EffSpec} {α : Type _} : (t : NodeTag E α) → (p : t.fields) → Type _
-| ret _, x => nomatch x
-| fail, x => nomatch x
-| tau, () => α
-| op _ _, Sum.inl _ => α
-| op e _, Sum.inr ⟨o, _⟩ => E.blockOutputs e o
-
-def Step (E : EffSpec) : Endo (Type _) where
-  Tag := fun α => NodeTag E α
-  Field := fun _=> NodeTag.fields
-  Elem := fun _ => NodeTag.elem
-
-namespace Step
-
-def ret {E α Y} (x : α) : Step E Y α := ⟨.ret x, fun a => PEmpty.elim a⟩
-def tau {E α Y} (x : Y α) : Step E Y α := ⟨.tau, fun () => x⟩
-def fail {E α Y} : Step E Y α := ⟨.fail, fun a => PEmpty.elim a⟩
-def op {E α Y} (e : E.tag) (inp : E.input e)
-    (blocks : (t : E.blockTag e) → E.blockInputs e t → Y (E.blockOutputs e t))
-    (k : (o : E.output e) → Y α) : Step E Y α :=
-  ⟨.op e inp, fun
-    | Sum.inl o => k o
-    | Sum.inr ⟨t, i⟩ => blocks t i
-  ⟩
-
-protected def casesOn {E Y} { motive : (α : Type _) → Step E Y α → Sort* } {α} (x : Step E Y α)
-    (ret : ∀ {α} x, motive α (ret x))
-    (tau : ∀ {α} x, motive α (tau x))
-    (fail : ∀ {α}, motive α fail)
-    (op : ∀ {α} e inp blocks k, motive α (op e inp blocks k)):
-    motive α x := by
-  rcases x with ⟨tag, fields⟩
-  cases tag with
-  | ret a =>
-    convert ret a
-    simp only [Step.ret]
-    congr 2
-    ext a; cases a
-  | tau =>
-    convert tau (fields ())
-    · rfl
-    · simp only [Step.tau]
-      congr
-  | fail =>
-    convert fail
-    simp only [Step.fail]
-    congr 2
-    ext a; cases a
-  | op e inp =>
-    convert op e inp (fun t i => fields (.inr ⟨t, i⟩)) (fun o => fields (.inl o))
-    simp only [Step.op]
-    congr 2
-    ext a; cases a <;> rfl
-
-@[simp]
-theorem map_ret {E} {Y Z : Type _ → Type _} {f : (α : Type _) → Y α → Z α} {α : Type _} {x : α}:
-    IxPoly.map (F := Step E) f α (Step.ret x) = Step.ret x := by
-  simp only [map, ret]
-  congr 1
-  ext a; cases a
-
-@[simp]
-theorem map_tau {E} {Y Z : Type _ → Type _} {f : (α : Type _) → Y α → Z α} {α : Type _} {x : Y α}:
-    IxPoly.map (F := Step E) f α (Step.tau x) = Step.tau (f α x) := by
-  simp only [map, tau]
-  congr 1
-
-@[simp]
-theorem map_fail {E} {Y Z : Type _ → Type _} {f : (α : Type _) → Y α → Z α} {α : Type _}:
-    IxPoly.map (F := Step E) f α (Step.fail) = Step.fail := by
-  simp only [map, fail]
-  congr 1
-  ext a; cases a
-
-@[simp]
-theorem map_op {E} {Y Z : Type _ → Type _} {f : (α : Type _) → Y α → Z α} {α : Type _}
-    {e : E.tag} {inp : E.input e}
-    {blocks : (t : E.blockTag e) → E.blockInputs e t → Y (E.blockOutputs e t)}
-    {k : (o : E.output e) → Y α}:
-    IxPoly.map (F := Step E) f α (Step.op e inp blocks k) =
-      Step.op e inp (fun t i => f _ (blocks t i)) (fun o => f _ (k o)) := by
-  simp only [map, op]
-  congr 1
-  ext a; cases a <;> rfl
-
-theorem tau_def {E} {Y : Type _ → Type _} {α : Type _} {x : Y α}:
-    Step.tau (E := E) x = ⟨.tau, fun _ => x⟩ := by rfl
-
-end Step
-
-end ITree
-
-def ITree (E : ITree.EffSpec) (α : Type _): Type _ := (ITree.Step E).M α
+def ITree (E : Eff.Spec) (α : Type _): Type _ := (Eff.Step E).M α
 namespace ITree
 
 open IxPoly
 
-def corec {E} {A : Type _ → Type _} (f : (i : Type _) → A i → Step E A i): {i : Type _} → A i → ITree E i :=
+def corec {E} {A : Type _ → Type _} (f : (i : Type _) → A i → Eff.Step E A i): {i : Type _} → A i → ITree E i :=
   IxPoly.M.corec f
 
-def observe {E α} : ITree E α ≃ Step E (ITree E) α := IxPoly.M.observe
+def observe {E α} : ITree E α ≃ Eff.Step E (ITree E) α := IxPoly.M.observe
 
-def roll {E α} : Step E (ITree E) α → ITree E α := IxPoly.M.observe.symm
+def roll {E α} : Eff.Step E (ITree E) α → ITree E α := IxPoly.M.observe.symm
 
-theorem observe_roll {E α} (x : Step E (ITree E) α): observe (roll x) = x := observe.apply_symm_apply _
+theorem observe_roll {E α} (x : Eff.Step E (ITree E) α): observe (roll x) = x := observe.apply_symm_apply _
 
 theorem roll_observe {E α} (x : ITree E α): roll (observe x) = x := observe.symm_apply_apply _
 
-theorem observe_corec {E} {A : Type _ → Type _} (f : (i : Type _) → A i → Step E A i) {i : Type _} (a : A i):
+theorem observe_corec {E} {A : Type _ → Type _} (f : (i : Type _) → A i → Eff.Step E A i) {i : Type _} (a : A i):
     observe (corec f a) = IxPoly.map (fun _ y => corec f y) i (f i a) := IxPoly.M.observe_corec
 
-def ret {E α} (x : α) : ITree E α := roll $ Step.ret x
-def tau {E α} (x : ITree E α) : ITree E α := roll $ Step.tau x
-def fail {E α} : ITree E α := roll $ Step.fail
+def ret {E α} (x : α) : ITree E α := roll $ Eff.Step.ret x
+def tau {E α} (x : ITree E α) : ITree E α := roll $ Eff.Step.tau x
+def fail {E α} : ITree E α := roll $ Eff.Step.fail
 def op {E α} (e : E.tag) (inp : E.input e)
     (blocks : (t : E.blockTag e) → E.blockInputs e t → ITree E (E.blockOutputs e t))
     (k : (o : E.output e) → ITree E α) : ITree E α :=
-  roll $ Step.op e inp blocks k
+  roll $ Eff.Step.op e inp blocks k
 
-theorem roll_ret {E α} (x : α) : roll (E:=E) (Step.ret x) = ret x := rfl
-theorem roll_tau {E α} (x : ITree E α) : roll (E:=E) (Step.tau x) = tau x := rfl
-theorem roll_fail {E α} : roll (E:=E) (α:=α) Step.fail = fail := rfl
+theorem roll_ret {E α} (x : α) : roll (E:=E) (Eff.Step.ret x) = ret x := rfl
+theorem roll_tau {E α} (x : ITree E α) : roll (E:=E) (Eff.Step.tau x) = tau x := rfl
+theorem roll_fail {E α} : roll (E:=E) (α:=α) Eff.Step.fail = fail := rfl
 theorem roll_op {E α} (e : E.tag) (inp : E.input e)
     (blocks : (t : E.blockTag e) → E.blockInputs e t → ITree E (E.blockOutputs e t))
     (k : (o : E.output e) → ITree E α) :
-    roll (E:=E) (Step.op e inp blocks k) = op e inp blocks k := rfl
+    roll (E:=E) (Eff.Step.op e inp blocks k) = op e inp blocks k := rfl
 
 @[simp]
-theorem observe_ret {E α} (x : α) : observe (ret x (E:=E)) = Step.ret x := rfl
+theorem observe_ret {E α} (x : α) : observe (ret x (E:=E)) = Eff.Step.ret x := rfl
 
 @[simp]
-theorem observe_tau {E α} (x : ITree E α) : observe (tau x (E:=E)) = Step.tau x := rfl
+theorem observe_tau {E α} (x : ITree E α) : observe (tau x (E:=E)) = Eff.Step.tau x := rfl
 
 @[simp]
-theorem observe_fail {E α} : observe (fail (E:=E) (α:=α)) = Step.fail := rfl
+theorem observe_fail {E α} : observe (fail (E:=E) (α:=α)) = Eff.Step.fail := rfl
 
 @[simp]
 theorem observe_op {E α} (e : E.tag) (inp : E.input e)
     (blocks : (t : E.blockTag e) → E.blockInputs e t → ITree E (E.blockOutputs e t))
     (k : (o : E.output e) → ITree E α) :
-    observe (op e inp blocks k (E:=E)) = Step.op e inp blocks k := rfl
+    observe (op e inp blocks k (E:=E)) = Eff.Step.op e inp blocks k := rfl
 
 protected def casesOn {E} { motive : (α : Type _) → ITree E α → Sort* } {α} (x : ITree E α)
     (ret : ∀ {α} x, motive α (ret x))
@@ -174,22 +61,22 @@ protected def casesOn {E} { motive : (α : Type _) → ITree E α → Sort* } {�
     motive α x := by
   have : x = roll (observe x) := (observe.symm_apply_apply _).symm
   rw [this]
-  cases observe x using Step.casesOn <;> apply_assumption
+  cases observe x using Eff.Step.casesOn <;> apply_assumption
 
 inductive BisimRelF {E}
     (R : (α : Type _) → ITree E α → ITree E α → Prop):
-    (α : Type _) → Step E (ITree E) α → Step E (ITree E) α → Prop where
-| ret {α} (x : α): BisimRelF R α (Step.ret x) (Step.ret x)
-| tau {α} (x y : ITree E α) (hr : R _ x y) : BisimRelF R α (Step.tau x) (Step.tau y)
-| fail {α} : BisimRelF R α Step.fail Step.fail
+    (α : Type _) → Eff.Step E (ITree E) α → Eff.Step E (ITree E) α → Prop where
+| ret {α} (x : α): BisimRelF R α (Eff.Step.ret x) (Eff.Step.ret x)
+| tau {α} (x y : ITree E α) (hr : R _ x y) : BisimRelF R α (Eff.Step.tau x) (Eff.Step.tau y)
+| fail {α} : BisimRelF R α Eff.Step.fail Eff.Step.fail
 | op {α} (e : E.tag) (inp : E.input e)
     (k1 k2 : (o : E.output e) → ITree E α)
     (blocks1 blocks2 : (t : E.blockTag e) → E.blockInputs e t → ITree E (E.blockOutputs e t))
     (h1 : ∀ o, R _ (k1 o) (k2 o))
     (h2 : ∀ t i, R _ (blocks1 t i) (blocks2 t i)):
-  BisimRelF R α (Step.op e inp blocks1 k1) (Step.op e inp blocks2 k2)
+  BisimRelF R α (Eff.Step.op e inp blocks1 k1) (Eff.Step.op e inp blocks2 k2)
 
-theorem BisimRelF.toLiftR {E} {R : (α : Type _) → ITree E α → ITree E α → Prop} : BisimRelF R ≤ IxPoly.M.LiftR (Step E) R := by
+theorem BisimRelF.toLiftR {E} {R : (α : Type _) → ITree E α → ITree E α → Prop} : BisimRelF R ≤ IxPoly.M.LiftR (Eff.Step E) R := by
   intro α x y hxy
   cases hxy <;> constructor
   case ret | fail => intro a; cases a
@@ -200,11 +87,11 @@ theorem BisimRelF.toLiftR {E} {R : (α : Type _) → ITree E α → ITree E α �
 
 theorem BisimRelF.refl {E R}
     (hrefl : ∀ {α} (x : ITree E α), R α x x)
-    {α} (x : Step E (ITree E) α): BisimRelF R α x x := by
-  cases x using Step.casesOn <;> constructor <;> intros <;> apply_assumption
+    {α} (x : Eff.Step E (ITree E) α): BisimRelF R α x x := by
+  cases x using Eff.Step.casesOn <;> constructor <;> intros <;> apply_assumption
 
 theorem BisimRelF.refl_upToEq {E R}
-    {α} (x : Step E (ITree E) α): BisimRelF (M.IxRel.upToEq R) α x x := by
+    {α} (x : Eff.Step E (ITree E) α): BisimRelF (M.IxRel.upToEq R) α x x := by
   apply BisimRelF.refl
   intros
   apply Or.inl
@@ -254,7 +141,7 @@ theorem bisim₂_up_to_eq {E α} {Seed : Type _ → Type _}
   exists seed
 
 def BindCarrier E α R := (ITree E α × (α → ITree E R)) ⊕ ITree E R
-def bindCo {E α} R : BindCarrier E α R → Step E (BindCarrier E α) R
+def bindCo {E α} R : BindCarrier E α R → Eff.Step E (BindCarrier E α) R
 | .inl (e, f) => match e.observe with
   | ⟨.ret x, _⟩ => IxPoly.map (fun _ => .inr) _ (f x).observe
   | ⟨.tau, cont⟩ => ⟨.tau, fun () => .inl (cont (), f)⟩
@@ -270,7 +157,7 @@ theorem bindCo_copy {E β} {x : ITree E β} : corec (bindCo (α := α)) (.inr x)
   intro _ x y hxy
   cases hxy
   · simp only [observe_corec, bindCo, IxPoly.map_map]
-    cases y.observe using Step.casesOn <;> {
+    cases y.observe using Eff.Step.casesOn <;> {
        try simp; constructor <;> { intros ; apply_assumption }
     }
   · rfl
@@ -283,18 +170,18 @@ instance {E} : Monad (ITree E) where
 theorem ret_bind {E β} {α} {x : α} {f : α → ITree E β} : ret x >>= f = f x := by
   apply observe.injective
   simp only [Bind.bind, observe_corec, bindCo, ret,
-    observe_roll, IxPoly.map_map, Step.ret, bindCo_copy, IxPoly.map_id]
+    observe_roll, IxPoly.map_map, Eff.Step.ret, bindCo_copy, IxPoly.map_id]
 
 @[simp]
 theorem tau_bind {E β} {α} {x : ITree E α} {f : α → ITree E β} : tau x >>= f = tau (x >>= f) := by
   apply observe.injective
-  simp only [Bind.bind, observe_corec, bindCo, tau, observe_roll, Step.tau, IxPoly.map]
+  simp only [Bind.bind, observe_corec, bindCo, tau, observe_roll, Eff.Step.tau, IxPoly.map]
   congr
 
 @[simp]
 theorem fail_bind {E β} {α} {f : α → ITree E β} : fail >>= f = fail := by
   apply observe.injective
-  simp only [Bind.bind, observe_corec, bindCo, fail, observe_roll, Step.fail, IxPoly.map]
+  simp only [Bind.bind, observe_corec, bindCo, fail, observe_roll, Eff.Step.fail, IxPoly.map]
   congr
   ext a
   cases a
@@ -310,7 +197,7 @@ theorem op_bind {E β} {α} {e : E.tag} {inp : E.input e}
         (fun o => k o >>= f) := by
   apply observe.injective
   simp only [Bind.bind, observe_corec, bindCo, op, observe_roll, IxPoly.map]
-  simp only [Step.op]
+  simp only [Eff.Step.op]
   congr
   ext a; cases a
   · rfl
@@ -367,17 +254,17 @@ instance {E} : LawfulMonad (ITree E) := LawfulMonad.mk' _
   (fun _ _ => ret_bind)
   (fun _ _ _ => bind_assoc)
 
-private def LoopCarrier (E : EffSpec) (β : Type _) (α : Type _) : Type _ :=
+private def LoopCarrier (E : Eff.Spec) (β : Type _) (α : Type _) : Type _ :=
     (ITree E (ForInStep β) × (β → ITree E α)) ⊕ ITree E α
 
-private def loopCo {E : EffSpec} {β : Type _} (body : β → ITree E (ForInStep β)) (α : Type _):
-  LoopCarrier E β α → Step E (LoopCarrier E β) α
+private def loopCo {E : Eff.Spec} {β : Type _} (body : β → ITree E (ForInStep β)) (α : Type _):
+  LoopCarrier E β α → Eff.Step E (LoopCarrier E β) α
 | .inl (m, f) => match m.observe with
   | ⟨.ret (.done v), _⟩ => IxPoly.map (fun _ => .inr) _ (f v).observe
-  | ⟨.ret (.yield v), _⟩ => Step.tau (.inl (body v, f))
-  | ⟨.tau, k⟩ => Step.tau (.inl (k (), f))
-  | ⟨.fail, _⟩ => Step.fail
-  | ⟨.op e inp, k⟩ => Step.op e inp
+  | ⟨.ret (.yield v), _⟩ => Eff.Step.tau (.inl (body v, f))
+  | ⟨.tau, k⟩ => Eff.Step.tau (.inl (k (), f))
+  | ⟨.fail, _⟩ => Eff.Step.fail
+  | ⟨.op e inp, k⟩ => Eff.Step.op e inp
       (fun t i => .inr (k $ .inr ⟨t, i⟩))
       (fun o => .inl (k $ .inl o, f))
 | .inr m => IxPoly.map (fun _ => .inr) _ m.observe
@@ -388,7 +275,7 @@ private theorem loopCo_copy {E β} {body : β → ITree E (ForInStep β)} {x : I
   intro _ x y hxy
   cases hxy
   · simp only [observe_corec, loopCo, IxPoly.map_map]
-    cases y.observe using Step.casesOn <;> {
+    cases y.observe using Eff.Step.casesOn <;> {
        try simp; constructor <;> { intros ; apply_assumption }
     }
   · rfl
@@ -417,15 +304,15 @@ theorem loop_def {E β α} {body : β → ITree E (ForInStep β)}
   cases x with
   | inr m =>
     simp only [observe_corec, loopCo, IxPoly.map_map]
-    cases m.observe using Step.casesOn with
+    cases m.observe using Eff.Step.casesOn with
     | ret | fail => simp [BisimRelF.refl_upToEq]
     | tau x =>
-      simp only [Step.map_tau]
+      simp only [Eff.Step.map_tau]
       apply BisimRelF.tau
       right
       exists (.inr x)
     | op e inp blocks k =>
-      simp only [Step.map_op]
+      simp only [Eff.Step.map_op]
       apply BisimRelF.op
       · intro o
         right
@@ -438,34 +325,34 @@ theorem loop_def {E β α} {body : β → ITree E (ForInStep β)}
     simp only
     have : m = roll (observe m) := (observe.symm_apply_apply _).symm
     rw [this]
-    cases m.observe using Step.casesOn with
+    cases m.observe using Eff.Step.casesOn with
     | ret x =>
       simp only [roll_ret, ret_bind]
       cases x with
       | done v =>
-        simp only [observe_corec, loopCo, observe_ret, Step.ret, map_map, loopCo_copy, IxPoly.map_id]
+        simp only [observe_corec, loopCo, observe_ret, Eff.Step.ret, map_map, loopCo_copy, IxPoly.map_id]
         apply BisimRelF.refl_upToEq
       | yield v =>
-        simp only [observe_tau, observe_corec, loopCo, observe_ret, Step.ret, Step.map_tau]
+        simp only [observe_tau, observe_corec, loopCo, observe_ret, Eff.Step.ret, Eff.Step.map_tau]
         apply BisimRelF.tau
         left
         rfl
     | fail =>
       simp only [roll_fail, observe_corec, loopCo, observe_fail, fail_bind]
-      conv => enter [3,3]; rw [Step.fail]
-      simp only [Step.map_fail]
+      conv => enter [3,3]; rw [Eff.Step.fail]
+      simp only [Eff.Step.map_fail]
       apply BisimRelF.fail
     | tau x =>
       simp only [roll_tau, observe_corec, loopCo, observe_tau, tau_bind]
-      conv => enter [3,3]; rw [Step.tau]
-      simp only [Step.map_tau]
+      conv => enter [3,3]; rw [Eff.Step.tau]
+      simp only [Eff.Step.map_tau]
       apply BisimRelF.tau
       right
       exists (.inl (x, f))
     | op e inp blocks k =>
       simp only [roll_op, observe_corec, loopCo, observe_op, op_bind]
-      conv => enter [3,3]; rw [Step.op]
-      simp only [Step.map_op]
+      conv => enter [3,3]; rw [Eff.Step.op]
+      simp only [Eff.Step.map_op]
       apply BisimRelF.op
       · intro o
         right
@@ -491,7 +378,7 @@ private theorem loopCo_bind {E β α}
   rcases seed with ⟨m, k⟩
   have hm : m = roll (observe m) := (observe.symm_apply_apply _).symm
   rw [hm]
-  cases observe m using Step.casesOn with
+  cases observe m using Eff.Step.casesOn with
   | ret x =>
     cases x with
     | done v =>
@@ -499,7 +386,7 @@ private theorem loopCo_bind {E β α}
           corec (loopCo body) (.inl (ret (.done v), f)) = f v := by
         intro j f
         apply observe.injective
-        simp only [observe_corec, loopCo, observe_ret, Step.ret, IxPoly.map_map,
+        simp only [observe_corec, loopCo, observe_ret, Eff.Step.ret, IxPoly.map_map,
           loopCo_copy, IxPoly.map_id]
       simp only [roll_ret]
       rw [unfold k, unfold pure]
@@ -511,7 +398,7 @@ private theorem loopCo_bind {E β α}
             tau (corec (loopCo body) (.inl (body v, f))) := by
         intro j f
         apply observe.injective
-        simp only [observe_corec, loopCo, observe_ret, Step.ret, Step.map_tau, observe_tau]
+        simp only [observe_corec, loopCo, observe_ret, Eff.Step.ret, Eff.Step.map_tau, observe_tau]
       simp only [roll_ret]
       rw [unfold k, unfold pure]
       simp only [tau_bind, observe_tau]
@@ -525,9 +412,9 @@ private theorem loopCo_bind {E β α}
       intro j f
       apply observe.injective
       have hco :
-          loopCo body j (.inl (tau next, f)) = Step.tau (.inl (next, f)) := by
-        simp only [loopCo, observe_tau, Step.tau]
-      rw [observe_corec, observe_tau, hco, Step.map_tau]
+          loopCo body j (.inl (tau next, f)) = Eff.Step.tau (.inl (next, f)) := by
+        simp only [loopCo, observe_tau, Eff.Step.tau]
+      rw [observe_corec, observe_tau, hco, Eff.Step.map_tau]
     simp only [roll_tau]
     rw [unfold k, unfold pure]
     simp only [tau_bind, observe_tau]
@@ -540,8 +427,8 @@ private theorem loopCo_bind {E β α}
       intro j f
       apply observe.injective
       rw [observe_corec, observe_fail]
-      change IxPoly.map (fun _ y => corec (loopCo body) y) _ Step.fail = _
-      simp only [Step.map_fail]
+      change IxPoly.map (fun _ y => corec (loopCo body) y) _ Eff.Step.fail = _
+      simp only [Eff.Step.map_fail]
     simp only [roll_fail]
     rw [unfold k, unfold pure]
     simp only [fail_bind, observe_fail]
@@ -554,12 +441,12 @@ private theorem loopCo_bind {E β α}
       apply observe.injective
       have hco :
           loopCo body j (.inl (op e inp blocks next, f)) =
-            Step.op e inp
+            Eff.Step.op e inp
               (fun t x => (.inr (blocks t x) : LoopCarrier E β (E.blockOutputs e t)))
               (fun o => .inl (next o, f)) := by
-        simp only [loopCo, observe_op, Step.op]
-      rw [observe_corec, observe_op, hco, Step.map_op]
-      congr
+        simp only [loopCo, observe_op, Eff.Step.op]
+      rw [observe_corec, observe_op, hco, Eff.Step.map_op]
+      congr 1
       funext t x
       exact loopCo_copy
     simp only [roll_op]
