Freigen/Eff.lean
@@ -1,0 +1,115 @@
+import Freigen.IxPoly.Basic
+
+namespace Freigen.Eff
+
+structure Spec where
+  tag : Type u
+  input : tag → Type v
+  output : tag → Type v
+  blockTag : tag → Type u
+  blockInputs : (t : tag) → blockTag t → Type v
+  blockOutputs : (t : tag) → blockTag t → Type v
+
+inductive NodeTag (E : Spec) : Type _ → Type _ where
+| ret {R} : R → NodeTag E R
+| tau {R} : NodeTag E R
+| fail {R} : NodeTag E R
+| op {R} (e : E.tag) : E.input e → NodeTag E R
+
+def NodeTag.fields {i} {E : Spec}: NodeTag E i → Type _
+| ret _ => PEmpty
+| tau => PUnit
+| fail => PEmpty
+| op e _ => E.output e ⊕ ((t : E.blockTag e) × E.blockInputs e t)
+
+def NodeTag.elem {E : Spec} {α : Type _} : (t : NodeTag E α) → (p : t.fields) → Type _
+| ret _, x => nomatch x
+| fail, x => nomatch x
+| tau, () => α
+| op _ _, Sum.inl _ => α
+| op e _, Sum.inr ⟨o, _⟩ => E.blockOutputs e o
+
+def Step (E : Spec) : IxPoly.Endo (Type _) where
+  Tag := fun α => NodeTag E α
+  Field := fun _=> NodeTag.fields
+  Elem := fun _ => NodeTag.elem
+
+namespace Step
+
+def ret {E α Y} (x : α) : Step E Y α := ⟨.ret x, fun a => PEmpty.elim a⟩
+def tau {E α Y} (x : Y α) : Step E Y α := ⟨.tau, fun () => x⟩
+def fail {E α Y} : Step E Y α := ⟨.fail, fun a => PEmpty.elim a⟩
+def op {E α Y} (e : E.tag) (inp : E.input e)
+    (blocks : (t : E.blockTag e) → E.blockInputs e t → Y (E.blockOutputs e t))
+    (k : (o : E.output e) → Y α) : Step E Y α :=
+  ⟨.op e inp, fun
+    | Sum.inl o => k o
+    | Sum.inr ⟨t, i⟩ => blocks t i
+  ⟩
+
+protected def casesOn {E Y} { motive : (α : Type _) → Step E Y α → Sort* } {α} (x : Step E Y α)
+    (ret : ∀ {α} x, motive α (ret x))
+    (tau : ∀ {α} x, motive α (tau x))
+    (fail : ∀ {α}, motive α fail)
+    (op : ∀ {α} e inp blocks k, motive α (op e inp blocks k)):
+    motive α x := by
+  rcases x with ⟨tag, fields⟩
+  cases tag with
+  | ret a =>
+    convert ret a
+    simp only [Step.ret]
+    congr 2
+    ext a; cases a
+  | tau =>
+    convert tau (fields ())
+    · rfl
+    · simp only [Step.tau]
+      congr
+  | fail =>
+    convert fail
+    simp only [Step.fail]
+    congr 2
+    ext a; cases a
+  | op e inp =>
+    convert op e inp (fun t i => fields (.inr ⟨t, i⟩)) (fun o => fields (.inl o))
+    simp only [Step.op]
+    congr 2
+    ext a; cases a <;> rfl
+
+@[simp]
+theorem map_ret {E} {Y Z : Type _ → Type _} {f : (α : Type _) → Y α → Z α} {α : Type _} {x : α}:
+    IxPoly.map (F := Step E) f α (Step.ret x) = Step.ret x := by
+  simp only [IxPoly.map, ret]
+  congr 1
+  ext a; cases a
+
+@[simp]
+theorem map_tau {E} {Y Z : Type _ → Type _} {f : (α : Type _) → Y α → Z α} {α : Type _} {x : Y α}:
+    IxPoly.map (F := Step E) f α (Step.tau x) = Step.tau (f α x) := by
+  simp only [IxPoly.map, tau]
+  congr 1
+
+@[simp]
+theorem map_fail {E} {Y Z : Type _ → Type _} {f : (α : Type _) → Y α → Z α} {α : Type _}:
+    IxPoly.map (F := Step E) f α (Step.fail) = Step.fail := by
+  simp only [IxPoly.map, fail]
+  congr 1
+  ext a; cases a
+
+@[simp]
+theorem map_op {E} {Y Z : Type _ → Type _} {f : (α : Type _) → Y α → Z α} {α : Type _}
+    {e : E.tag} {inp : E.input e}
+    {blocks : (t : E.blockTag e) → E.blockInputs e t → Y (E.blockOutputs e t)}
+    {k : (o : E.output e) → Y α}:
+    IxPoly.map (F := Step E) f α (Step.op e inp blocks k) =
+      Step.op e inp (fun t i => f _ (blocks t i)) (fun o => f _ (k o)) := by
+  simp only [IxPoly.map, op]
+  congr 1
+  ext a; cases a <;> rfl
+
+theorem tau_def {E} {Y : Type _ → Type _} {α : Type _} {x : Y α}:
+    Step.tau (E := E) x = ⟨.tau, fun _ => x⟩ := by rfl
+
+end Step
+
+end Freigen.Eff
