Freigen/Free.lean
@@ -1,0 +1,74 @@
+import Freigen.IxPoly.Defs
+import Freigen.ExactCodensity
+import Freigen.Eff
+
+namespace Freigen
+
+def wBind {α β} {E} (a : IxPoly.W (Eff.Step E) α) (f : α → IxPoly.W (Eff.Step E) β): IxPoly.W (Eff.Step E) β := match a with
+  | IxPoly.W.mk i p g => match p with
+    | .ret a => f a
+    | .tau => IxPoly.W.roll (Eff.Step.tau $ wBind (g ()) f)
+    | .fail => IxPoly.W.roll (Eff.Step.fail)
+    | .op e inp => IxPoly.W.mk (F := Eff.Step E) _ (Eff.NodeTag.op e inp) (fun
+      | .inl a => wBind (g (.inl a)) f
+      | .inr b => g (.inr b)
+    )
+
+instance {E} : Monad (IxPoly.W (Eff.Step E)) where
+  pure a := IxPoly.W.roll (Eff.Step.ret a)
+  bind x f := wBind x f
+
+instance {E} : LawfulMonad (IxPoly.W (Eff.Step E)) := LawfulMonad.mk' _
+  (by
+    intro _ x
+    change wBind x (fun a => IxPoly.W.roll (Eff.Step.ret a)) = x
+    induction x with
+    | mk i p g ih =>
+      cases p
+      · simp [wBind, IxPoly.W.roll, Eff.Step.ret]
+        ext a
+        cases a
+      · have := ih ()
+        simp only [wBind, IxPoly.W.roll, Eff.Step.tau]
+        simp only [IxPoly.W.roll] at this
+        simp only [IxPoly.W.mk.injEq, heq_eq_eq, true_and]
+        ext x; cases x
+        simp only
+        exact this
+      · simp [wBind, IxPoly.W.roll, Eff.Step.fail]
+        ext x; cases x;
+      · simp only [wBind]
+        congr
+        ext x
+        cases x
+        · simp only
+          apply_assumption
+        · rfl
+  )
+  (by intros; rfl)
+  (by
+    intro _ _ _ a f g
+    induction a with
+    | mk i p g ih =>
+      cases p
+      · rfl
+      · simp only [Bind.bind, wBind, Eff.Step.tau, IxPoly.W.roll]
+        congr 1
+        ext x; cases x
+        simp only
+        apply ih
+      · simp only [Bind.bind, wBind, Eff.Step.fail, IxPoly.W.roll]
+      · simp only [Bind.bind, wBind]
+        congr
+        ext x; cases x
+        · simp only
+          apply ih
+        · rfl
+  )
+
+def Free (E : Eff.Spec) (α : Type) : Type _ := ExactCodensity (IxPoly.W (Eff.Step E)) α
+
+instance {E} : Monad (Free E) := inferInstanceAs (Monad (ExactCodensity (IxPoly.W (Eff.Step E))))
+instance {E} : LawfulMonad (Free E) := inferInstanceAs (LawfulMonad (ExactCodensity (IxPoly.W (Eff.Step E))))
+
+end Freigen
